theories/gitree/lambda.v
@@ -10,49 +10,98 @@ Section lambda.
 
   Notation IT := (IT Σ A).
 
-  Program Definition IF `{!SubOfe natO A} : IT -n> IT -n> IT -n> IT := λne t t1 t2,
+  Program Definition IF_ne `{!SubOfe natO A} : IT -n> IT -n> IT -n> IT := λne t t1 t2,
       get_ret (λne n, if Nat.ltb 0 n then t1 else t2) t.
   Next Obligation. repeat intro. by rewrite H. Qed.
   Solve All Obligations with solve_proper_please.
 
-  Program Definition IF_last `{!SubOfe natO A} : IT -n> IT -n> IT -n> IT := λne t1 t2 t, IF t t1 t2.
-  Solve All Obligations with solve_proper_please.
+  Definition IF `{!SubOfe natO A} x y z := IF_ne x y z.
+  Global Instance IF_Proper `{H : !SubOfe natO A}
+    : Proper ((≡) ==> (≡) ==> (≡) ==> (≡)) (@IF H).
+  Proof. rewrite /IF; solve_proper_please. Qed.
+  Global Instance IF_NonExp `{H : !SubOfe natO A} : NonExpansive3 (@IF H).
+  Proof. rewrite /IF; solve_proper_please. Qed.
+
+  Program Definition IF_last_ne `{!SubOfe natO A} : IT -n> IT -n> IT -n> IT := λne t1 t2 t, IF t t1 t2.
+  Solve All Obligations with rewrite /IF; solve_proper_please.
+  Definition IF_last `{!SubOfe natO A} x y z := IF_last_ne x y z.
+  Global Instance IF_last_Proper `{H : !SubOfe natO A}
+    : Proper ((≡) ==> (≡) ==> (≡) ==> (≡)) (@IF_last H).
+  Proof. rewrite /IF_last; solve_proper_please. Qed.
+  Global Instance IF_last_NonExp `{H : !SubOfe natO A} : NonExpansive3 (@IF_last H).
+  Proof. rewrite /IF_last; solve_proper_please. Qed.
 
   (** A non-strict application, does not recurse under the effects of the argument *)
-  Program Definition APP : IT -n> laterO IT -n> IT := λne f x,
+  Program Definition APP_ne : IT -n> laterO IT -n> IT := λne f x,
       get_fun (λne f, Tau $ laterO_ap f x) f.
   Solve All Obligations with solve_proper_please.
+  Definition APP x y := APP_ne x y.
+  Global Instance APP_Proper
+    : Proper ((≡) ==> (≡) ==> (≡)) APP.
+  Proof. rewrite /APP; solve_proper_please. Qed.
+  Global Instance APP_NonExp : NonExpansive2 APP.
+  Proof. rewrite /APP; solve_proper_please. Qed.
 
-  Program Definition Ppa : laterO IT -n> IT -n> IT := λne x f, APP f x.
-  Solve All Obligations with solve_proper_please.
+  Program Definition Ppa_ne : laterO IT -n> IT -n> IT := λne x f, APP f x.
+  Solve All Obligations with rewrite /APP; solve_proper_please.
+  Definition Ppa x y := Ppa_ne x y.
+  Global Instance Ppa_Proper
+    : Proper ((≡) ==> (≡) ==> (≡)) Ppa.
+  Proof. rewrite /Ppa; solve_proper_please. Qed.
+  Global Instance Ppa_NonExp : NonExpansive2 Ppa.
+  Proof. rewrite /Ppa; solve_proper_please. Qed.
 
   (** Strict version of APP *)
-  Program Definition APP' : IT -n> IT -n> IT := λne f, get_val (APP f ◎ NextO).
+  Program Definition APP'_ne : IT -n> IT -n> IT := λne f, get_val (APP_ne f ◎ NextO).
   Solve All Obligations with solve_proper_please.
+  Definition APP' x y := APP'_ne x y.
+  Global Instance APP'_Proper
+    : Proper ((≡) ==> (≡) ==> (≡)) APP'.
+  Proof. rewrite /APP'; solve_proper_please. Qed.
+  Global Instance APP'_NonExp : NonExpansive2 APP'.
+  Proof. rewrite /APP'; solve_proper_please. Qed.
 
   (** We define the interpretation of NatOp in two stages.
       First, we recurse under ticks and visitors in both arguments, and only then perform the op
    *)
-  Program Definition NATOP `{!SubOfe natO A} (f : nat → nat → nat) : IT -n> IT -n> IT := λne t1 t2,
+  Program Definition NATOP_ne `{!SubOfe natO A} (f : nat → nat → nat) : IT -n> IT -n> IT := λne t1 t2,
       get_val (λne v2,
         get_val (λne v1,
                    get_ret2 (λne n1 n2, Ret (f n1 n2)) v1 v2) t1) t2.
   Solve All Obligations with solve_proper_please.
+  Definition NATOP `{!SubOfe natO A} f x y := NATOP_ne f x y.
+  Global Instance NATOP_Proper `{H : !SubOfe natO A} f
+    : Proper ((≡) ==> (≡) ==> (≡)) (@NATOP H f).
+  Proof. rewrite /NATOP; solve_proper_please. Qed.
+  Global Instance NATOP_NonExp `{H : !SubOfe natO A} f : NonExpansive2 (@NATOP H f).
+  Proof. rewrite /NATOP; solve_proper_please. Qed.
 
   (** Sequencing *)
-  Program Definition SEQ : IT -n> IT -n> IT := λne α β,
+  Program Definition SEQ_ne : IT -n> IT -n> IT := λne α β,
       get_val (constO β) α.
   Solve Obligations with solve_proper_please.
+  Definition SEQ x y := SEQ_ne x y.
+  Global Instance SEQ_Proper
+    : Proper ((≡) ==> (≡) ==> (≡)) SEQ.
+  Proof. rewrite /SEQ; solve_proper_please. Qed.
+  Global Instance SEQ_NonExp : NonExpansive2 SEQ.
+  Proof. rewrite /SEQ; solve_proper_please. Qed.
 
-  Program Definition LET : IT -n> (IT -n> IT) -n> IT := λne x f, get_val f x.
+  Program Definition LET_ne : IT -n> (IT -n> IT) -n> IT := λne x f, get_val f x.
   Solve Obligations with solve_proper.
+  Definition LET x y := LET_ne x y.
+  Global Instance LET_Proper
+    : Proper ((≡) ==> (≡) ==> (≡)) LET.
+  Proof. rewrite /LET; intros f g Hfg x y Hxy; solve_proper. Qed.
+    Global Instance LET_NonExp : NonExpansive2 LET.
+  Proof. rewrite /LET; intros n f g Hfg x y Hxy; solve_proper. Qed.
 
   Lemma APP_Ret x y : APP (core.Ret x) y ≡ Err RuntimeErr.
-  Proof. simpl. by rewrite core.get_fun_ret. Qed.
+  Proof. simpl. by rewrite /APP /APP_ne //= core.get_fun_ret. Qed.
   Lemma APP_Err e x : APP (Err e) x ≡ Err e.
-  Proof. simpl. by rewrite get_fun_err. Qed.
+  Proof. simpl. by rewrite /APP /APP_ne //= get_fun_err. Qed.
   Lemma APP_Fun f x : APP (Fun f) x ≡ Tau $ laterO_ap f x.
-  Proof. simpl. rewrite get_fun_fun. done. Qed.
+  Proof. simpl. by rewrite /APP /APP_ne //= get_fun_fun. Qed.
   Lemma APP_Tick t x : APP (Tick t) x ≡ Tick $ APP t x.
   Proof.
      rewrite {1}/APP /=.
@@ -62,26 +111,26 @@ Section lambda.
   Proof.
     induction n; eauto. rewrite APP_Tick. rewrite IHn. done.
   Qed.
-  Lemma APP_Vis op i k x : APP (Vis op i k) x ≡ Vis op i (laterO_map (Ppa x) ◎ k).
+  Lemma APP_Vis op i k x : APP (Vis op i k) x ≡ Vis op i (laterO_map (Ppa_ne x) ◎ k).
   Proof.
     rewrite {1}/APP /=.
     rewrite get_fun_vis. repeat f_equiv.
     intro f. simpl. reflexivity.
   Qed.
   Lemma APP'_Err_r f e : APP' f (Err e) ≡ Err e.
-  Proof. simpl. by rewrite get_val_err. Qed.
+  Proof. simpl. by rewrite /APP' /APP'_ne //= get_val_err. Qed.
   Lemma APP'_Ret_r f x : APP' f (core.Ret x) ≡ APP f (Next (core.Ret x)).
-  Proof. simpl. rewrite core.get_val_ret. done. Qed.
+  Proof. simpl. by rewrite /APP' /APP'_ne //= core.get_val_ret. Qed.
   Lemma APP'_Fun_r f x : APP' f (Fun x) ≡ APP f (Next (Fun x)).
-  Proof. simpl. rewrite get_val_fun. done. Qed.
+  Proof. simpl. by rewrite /APP' /APP'_ne //= get_val_fun. Qed.
   Lemma APP'_Tick_r f t : APP' f (Tick t) ≡ Tick $ APP' f t.
-  Proof. by rewrite get_val_tick. Qed.
+  Proof. by rewrite /APP' /APP'_ne //= get_val_tick. Qed.
   Lemma APP'_Tick_r_n  f n t : APP' f (Tick_n n t) ≡ Tick_n n $ APP' f t.
   Proof.
     induction n; eauto. by rewrite APP'_Tick_r IHn.
   Qed.
   Lemma APP'_Vis_r f op i k : APP' f (Vis op i k) ≡ Vis op i (laterO_map (APP' f) ◎ k).
-  Proof. by rewrite get_val_vis. Qed.
+  Proof. by rewrite /APP' /APP'_ne //= get_val_vis. Qed.
   Lemma APP_APP'_ITV' α (βv : ITV Σ A) :
     APP' α (IT_of_V βv) ≡ APP α (Next (IT_of_V βv)).
   Proof.
@@ -97,7 +146,7 @@ Section lambda.
     rewrite APP_APP'_ITV'//.
   Qed.
   Lemma APP'_Vis_l β op i k `{!AsVal β} :
-    APP' (Vis op i k) β ≡ Vis op i (laterO_map (flipO APP' β) ◎ k).
+    APP' (Vis op i k) β ≡ Vis op i (laterO_map (flipO APP'_ne β) ◎ k).
   Proof.
     rewrite APP_APP'_ITV.
     rewrite APP_Vis. repeat f_equiv.
@@ -141,7 +190,7 @@ Section lambda.
     induction n; eauto. by rewrite IF_Tick IHn.
   Qed.
   Lemma IF_Vis `{!SubOfe natO A} op i k t1 t2 :
-    IF (Vis op i k) t1 t2 ≡ Vis op i (laterO_map (IF_last t1 t2) ◎ k).
+    IF (Vis op i k) t1 t2 ≡ Vis op i (laterO_map (IF_last_ne t1 t2) ◎ k).
   Proof.
     rewrite {1}/IF /=.
     rewrite get_ret_vis. repeat f_equiv.
@@ -149,17 +198,17 @@ Section lambda.
   Qed.
 
   Lemma NATOP_Err_r `{!SubOfe natO A} f e t1 : NATOP f t1 (Err e) ≡ Err e.
-  Proof. simpl. by rewrite get_val_err. Qed.
+  Proof. simpl. by rewrite /NATOP /NATOP_ne //= get_val_err. Qed.
   Lemma NATOP_Err_l `{!SubOfe natO A} f e β : AsVal β → NATOP f (Err e) β ≡ Err e.
   Proof.
     intros ?. simpl.
-    rewrite get_val_ITV /= get_val_err //.
+    rewrite /NATOP /NATOP_ne //= get_val_ITV /= get_val_err //.
   Qed.
   Lemma NATOP_Ret `{!SubOfe natO A} n1 n2 f :
     NATOP f (Ret n1) (Ret n2) ≡ Ret (f n1 n2).
   Proof.
     simpl.
-    rewrite get_val_ret/= get_val_ret/=.
+    rewrite /NATOP /NATOP_ne /= get_val_ret/= get_val_ret/=.
     rewrite !get_ret_ret. simpl.
     rewrite !get_ret_ret. simpl.
     done.
@@ -167,7 +216,7 @@ Section lambda.
   Lemma NATOP_Tick_r `{!SubOfe natO A} t1 t2 f :
     NATOP f t1 (Tick t2) ≡ Tick $ NATOP f t1 t2.
   Proof.
-    simpl. rewrite get_val_tick//.
+    simpl. rewrite /NATOP /NATOP_ne /= get_val_tick//.
   Qed.
   Lemma NATOP_Tick_n_r `{!SubOfe natO A} t1 t2 f n :
     NATOP f t1 (Tick_n n t2) ≡ Tick_n n $ NATOP f t1 t2.
@@ -179,7 +228,7 @@ Section lambda.
     AsVal β →
     NATOP f (Tick t1) β ≡ Tick $ NATOP f t1 β.
   Proof.
-    intros ?. simpl. rewrite get_val_ITV/=.
+    intros ?. simpl. rewrite /NATOP /NATOP_ne /= get_val_ITV/=.
     rewrite get_val_tick. f_equiv.
     rewrite get_val_ITV. done.
   Qed.
@@ -192,16 +241,16 @@ Section lambda.
     rewrite IHn. done.
   Qed.
   Lemma NATOP_Vis_r `{!SubOfe natO A} t1 op i k f :
-    NATOP f t1 (Vis op i k) ≡ Vis op i (laterO_map (NATOP f t1) ◎ k).
+    NATOP f t1 (Vis op i k) ≡ Vis op i (laterO_map (NATOP_ne f t1) ◎ k).
   Proof.
-    simpl. rewrite get_val_vis. f_equiv. solve_proper.
+    simpl. rewrite /NATOP /NATOP_ne /= get_val_vis. f_equiv. solve_proper.
   Qed.
   Lemma NATOP_ITV_Vis_l `{!SubOfe natO A} op i k β f :
     AsVal β →
     NATOP f (Vis op i k) β ≡
-    Vis op i (laterO_map (flipO (NATOP f) β) ◎ k).
+    Vis op i (laterO_map (flipO (NATOP_ne f) β) ◎ k).
   Proof.
-    intros ?. simpl. rewrite get_val_ITV/=.
+    intros ?. simpl. rewrite /NATOP /NATOP_ne /= get_val_ITV/=.
     rewrite get_val_vis. repeat f_equiv.
     intro y. simpl. rewrite get_val_ITV//.
   Qed.
@@ -210,15 +259,6 @@ Section lambda.
   Proof. unfold SEQ. simpl. rewrite get_val_ITV//. Qed.
   Lemma LET_Val α f `{!AsVal α} : LET α f ≡ f α.
   Proof. unfold LET. simpl. rewrite get_val_ITV//. Qed.
-
-  Global Instance IF_Proper `{!SubOfe natO A} : Proper ((≡) ==> (≡)) IF.
-  Proof. apply ne_proper. apply _. Qed.
-  Global Instance APP_Proper : Proper ((≡) ==> (≡)) APP.
-  Proof. apply ne_proper. apply _. Qed.
-  Global Instance APP'_Proper : Proper ((≡) ==> (≡)) APP'.
-  Proof. apply ne_proper. apply _. Qed.
-  Global Instance NATOP_Proper `{!SubOfe natO A} f : Proper ((≡) ==> (≡)) (NATOP f).
-  Proof. apply ne_proper. apply _. Qed.
 
   Opaque APP APP' IF NATOP.
   Definition AppLSCtx (β α : IT) := APP' α β.
@@ -245,6 +285,7 @@ Section lambda.
   Proof.
     unfold AppRSCtx.
     simple refine (IT_HOM _ _ _ _ _); simpl.
+    - solve_proper.
     - intros a. by rewrite APP'_Tick_r.
     - intros op i k. rewrite APP'_Vis_r. repeat f_equiv.
       by intro.
@@ -267,8 +308,7 @@ Section lambda.
   #[local] Instance NatOpRSCtx_ne op (β : IT) `{!SubOfe natO A} : NonExpansive (NatOpRSCtx op β).
   Proof.
     intro n. unfold NatOpRSCtx.
-    repeat intro. by apply (NATOP _ β).
-    (* XXX why doesn't f_equiv work here? *)
+    solve_proper.
   Qed.
   #[export] Instance NatOpRSCtx_hom op (β : IT) `{!SubOfe natO A} : IT_hom (NatOpRSCtx op β).
   Proof.
@@ -313,4 +353,3 @@ Notation "'λit' x .. y , P" := (Fun (Next (λne x, .. (Fun (Next (λne y, P))) 
 
 Notation "f ⊙ x" := (APP' f x)
                       (at level 10,  left associativity).
-
