theories/hom.v
@@ -12,38 +12,55 @@ Section hom.
   Notation IT := (IT F A).
   Notation ITV := (ITV F A).
 
-  Definition HOM : ofe := @sigO (IT -n> IT) IT_hom.
+  Record HOM_Type : Type :=
+    MkHom {
+        hom_fun :> IT -> IT;
+        hom_is_hom : IT_hom hom_fun;
+      }.
 
-  Global Instance HOM_hom (κ : HOM) : IT_hom (`κ).
+  Global Instance HOM_proper (f : HOM_Type) : Proper ((≡) ==> (≡)) f.
+  Proof. apply ne_proper, hom_is_hom. Qed.
+  Local Instance HOM_equiv : Equiv HOM_Type := λ f g, ∀ x, f x ≡ g x.
+  Local Instance HOM_dist : Dist HOM_Type := λ n f g, ∀ x, f x ≡{n}≡ g x.
+  Definition HOM_ofe_mixin : OfeMixin HOM_Type.
   Proof.
-    apply (proj2_sig κ).
+    split.
+    - intros f g; split; [intros Hfg n k; apply equiv_dist, Hfg|].
+      intros Hfg k.
+      apply equiv_dist; intros n; apply Hfg.
+    - intros n; split.
+      + by intros f x.
+      + by intros f g ? x.
+      + by intros f g h ?? x; trans (g x).
+    - intros n m f g ? x ?; eauto using dist_le with si_solver.
   Qed.
+  Canonical Structure HOM := Ofe HOM_Type HOM_ofe_mixin.
 
-  Program Definition HOM_id : HOM := exist _ idfun _.
-  Next Obligation.
-    apply _.
-  Qed.
+  Global Instance HOM_hom (κ : HOM) : IT_hom κ.
+  Proof. apply (hom_is_hom κ). Qed.
+
+  Definition HOM_id : HOM := MkHom idfun _.
 
   Lemma HOM_ccompose (f g : HOM) :
-    ∀ α, `f (`g α) = (`f ◎ `g) α.
+    ∀ α, f (g α) = (f ∘ g) α.
   Proof.
     intro; reflexivity.
   Qed.
 
-  Program Definition HOM_compose (f g : HOM) : HOM := exist _ (`f ◎ `g) _.
-  Next Obligation.
-    intros f g; simpl.
-    apply _.
-  Qed.
+  Definition HOM_compose (f g : HOM) : HOM := MkHom (f ∘ g) _.
 
   Lemma HOM_compose_ccompose (f g h : HOM) :
     h = HOM_compose f g ->
-    `f ◎ `g = `h.
+    f ∘ g = h.
   Proof. intros ->. done. Qed.
 
-  Program Definition IFSCtx_HOM `{!SubOfe natO A} α β : HOM := exist _ (λne x, IFSCtx α β x) _.
-  Next Obligation.
-    intros; simpl.
-    apply _.
-  Qed.
+  Definition IFSCtx_HOM `{!SubOfe natO A} α β : HOM := MkHom (λ x, IFSCtx α β x) _.
+
+  Program Definition LET_HOM (f : IT -n> IT) : HOM
+    := MkHom (LETCTX f) (LETCTX_Hom f).
+
+  Lemma LET_HOM_eq α (f : IT -n> IT)
+    : LET α f ≡ (LET_HOM f) α.
+  Proof. reflexivity. Qed.
+
 End hom.
