theories/lib/iter.v
@@ -40,14 +40,14 @@ Section iter.
     - repeat f_equiv. apply (fixpoint_unfold pre_iter).
     - trans (Tick (pre_iter_2 ITER f ⊙ α ⊙ β)).
       { unfold pre_iter.
-        rewrite -APP'_Tick_l. do 2 f_equiv.
-        rewrite -APP'_Tick_l. do 2 f_equiv.
+        rewrite -APP'_Tick_l. f_equiv.
+        rewrite -APP'_Tick_l. f_equiv.
         rewrite APP'_Fun_l. cbn-[pre_iter_2].
         by rewrite Tick_eq. }
       rewrite Tick_n_S. f_equiv.
       trans (Tick (pre_iter_1 ITER f α ⊙ β)).
       { unfold pre_iter_2.
-        rewrite -APP'_Tick_l. do 2 f_equiv.
+        rewrite -APP'_Tick_l. f_equiv.
         rewrite APP'_Fun_l. cbn-[pre_iter_2].
         by rewrite Tick_eq. }
       rewrite Tick_n_S. f_equiv.
