theories/utils/wbwp.v
@@ -1,0 +1,340 @@
+(* This file is copied and adapted from the weakestpre file in the iris development. *)
+
+From stdpp Require Export coPset.
+From iris.proofmode Require Import base proofmode classes.
+From iris.base_logic.lib Require Export fancy_updates.
+From gitrees Require Export prelude gitree lang_generic hom.
+Require Export gitrees.gitree.weakestpre.
+From gitrees Require Export utils.ghost_stacks utils.clwp.
+Import uPred.
+
+Section wbwp.
+  Context {n : nat} {a : is_ctx_dep} (rs : gReifiers a n) {A} `{!Cofe A}.
+  Notation rG := (gReifiers_sReifier rs).
+  Notation F := (sReifier_ops rG).
+  Notation IT := (IT F A).
+  Notation ITV := (ITV F A).
+  Notation stateF := (gReifiers_state rs).
+  Notation stateO := (stateF ♯ IT).
+  Notation stateR := (gReifiers_ucmra rs IT).
+  Let of_state := (of_state rs IT).
+  Let of_idx := (of_idx rs IT).
+  Notation reify := (reify rG).
+  Notation istep := (istep rG).
+  Notation isteps := (isteps rG).
+  Notation sstep := (sstep rG).
+  Notation ssteps := (ssteps rG).
+
+  Implicit Type op : opid F.
+  Implicit Type α β : IT.
+
+  Context `{!invGS Σ} `{!stateG rs A Σ}.
+  Notation iProp := (iProp Σ).
+  Notation coPsetO := (leibnizO coPset).
+
+  Program Definition wbwp `{!gstacksIG Σ}
+    (E : coPset) (out : gset ghost_id)
+    (e : IT) (Φ : ITV -n> iProp) : iProp
+    :=
+    ∀ M, gstacks_except M out
+         -∗ CLWP@{rs} e @ E {{v, ∃ N, ⌜M ⊆ N⌝ ∗ gstacks_except N out ∗ Φ v}}.
+  Next Obligation.
+    solve_proper.
+  Qed.
+
+  Global Typeclasses Opaque wbwp.
+End wbwp.
+
+(** Notations for partial weakest preconditions *)
+(** Notations without binder -- only parsing because they overlap with the
+notations with binder. *)
+Notation "'WBWP@{' re } e @ out ; E {{ Φ } }" := (wbwp re E out e Φ)
+  (at level 20, e, Φ at level 200, only parsing) : bi_scope.
+Notation "'WBWP@{' re } e @ E {{ Φ } }" := (wbwp re E ∅ e Φ)
+  (at level 20, e, Φ at level 200, only parsing) : bi_scope.
+Notation "'WBWP@{' re } e {{ Φ } }" := (wbwp re ⊤ ∅ e Φ)
+  (at level 20, e, Φ at level 200, only parsing) : bi_scope.
+Notation "'WBWP@{' re } e '@<' out >{{ Φ } }" := (wbwp re ⊤ out e Φ)
+  (at level 20, e, Φ at level 200, only parsing) : bi_scope.
+
+Notation "'WBWP@{' re } e @ out ; E {{ v , Q } }" := (wbwp re E out e (λne v, Q))
+  (at level 20, e, Q at level 200,
+   format "'[hv' 'WBWP@{' re }  e  '/' @  '[' out ;  '/' E  ']' '/' {{  '[' v ,  '/' Q  ']' } } ']'") : bi_scope.
+Notation "'WBWP@{' re } e @ E {{ v , Q } }" := (wbwp re E ∅ e (λne v, Q))
+  (at level 20, e, Q at level 200,
+   format "'[hv' 'WBWP@{' re }  e  '/' @  E  '/' {{  '[' v ,  '/' Q  ']' } } ']'") : bi_scope.
+Notation "'WBWP@{' re } e {{ v , Q } }" := (wbwp re ⊤ ∅ e (λne v, Q))
+  (at level 20, e, Q at level 200,
+   format "'[hv' 'WBWP@{' re }  e  '/' {{  '[' v ,  '/' Q  ']' } } ']'") : bi_scope.
+Notation "'WBWP@{' re } e '@<' out >{{ v , Q } }" := (wbwp re ⊤ out e (λne v, Q))
+  (at level 20, e, Q at level 200,
+   format "'[hv' 'WBWP@{' re }  e  '/' '@<'  out  >{{  '[' v ,  '/' Q  ']' } } ']'") : bi_scope.
+
+Section wp.
+  Context {n : nat} {a : is_ctx_dep} (rs : gReifiers a n) {A} `{!Cofe A}.
+  Notation rG := (gReifiers_sReifier rs).
+  Notation F := (sReifier_ops rG).
+  Notation IT := (IT F A).
+  Notation ITV := (ITV F A).
+  Notation stateF := (gReifiers_state rs).
+  Notation stateO := (stateF ♯ IT).
+  Notation stateR := (gReifiers_ucmra rs IT).
+  Let of_state := (of_state rs IT).
+  Let of_idx := (of_idx rs IT).
+  Notation reify := (reify rG).
+  Notation istep := (istep rG).
+  Notation isteps := (isteps rG).
+  Notation sstep := (sstep rG).
+  Notation ssteps := (ssteps rG).
+
+  Implicit Type op : opid F.
+  Implicit Type α β : IT.
+
+  Context `{!invGS Σ} `{!stateG rs A Σ} `{!gstacksIG Σ}.
+  Notation iProp := (iProp Σ).
+  Notation coPsetO := (leibnizO coPset).
+
+  Global Instance wbwp_ne E out m :
+    Proper ((dist m) ==> (dist m) ==> (dist m)) (wbwp rs E out).
+  Proof.
+    intros ??????; rewrite /wbwp /=.
+    f_equiv; intro; simpl.
+    repeat f_equiv; first done.
+    intro; simpl.
+    solve_proper.
+  Qed.
+  Global Instance wbwp_proper E out :
+    Proper ((≡) ==> (≡) ==> (≡)) (wbwp rs E out).
+  Proof.
+    intros ??? Φ Φ' ?. apply equiv_dist=>m.
+    by apply wbwp_ne; apply equiv_dist.
+  Qed.
+
+  Lemma wbwp_value_fupd' E out (Φ : ITV -n> iProp) v :
+    (|={E}=> Φ v) ⊢ WBWP@{rs} (IT_of_V v) @ out; E {{ Φ }}.
+  Proof.
+    rewrite /wbwp; iIntros ">?" (?) "?"; iApply clwp_value_fupd';
+      iExists _; iFrame; done.
+  Qed.
+
+
+  Lemma wbwp_val s E (Φ : ITV -n> iProp) α αv `{!IntoVal α αv}
+    : (|={E}=> Φ αv) ⊢ WBWP@{rs} α @ s ; E {{ Φ }}.
+  Proof.
+    iIntros "G".
+    rewrite -(into_val (α := α)).
+    by iApply wbwp_value_fupd'.
+  Qed.
+
+  Lemma wbwp_mono E out e (Φ Ψ : ITV -n> iProp) :
+    WBWP@{rs} e @ out; E {{ Φ }} -∗ (∀ v, Φ v ={E}=∗ Ψ v) -∗ WBWP@{rs} e @ out; E {{ Ψ }}.
+  Proof.
+    iIntros "H HΦ".
+    rewrite /wbwp.
+    iIntros (M) "HM".
+    iApply (clwp_mono with "[H HM]"); [iApply "H"|]; [iApply "HM"|].
+    iIntros (?); iDestruct 1 as (?) "[? [? ?]]".
+    iMod ("HΦ" with "[$]").
+    iModIntro; iExists _; iFrame.
+  Qed.
+
+  Lemma wbwp_get_gstack_full m E out e (Φ : ITV -n> iProp) :
+    m ∉ out →
+    gstack_exists m
+    -∗ (∀ s, gstack_full m s -∗ WBWP@{rs} e @ (out ∪ {[m]}); E {{v, gstack_full m s ∗ Φ v }})
+    -∗ WBWP@{rs} e @ out; E {{ Φ }}.
+  Proof.
+    iIntros (?) "#Hex HWBWP".
+    rewrite /wbwp.
+    iIntros (M) "HM".
+    iDestruct (gstack_exists_in with "Hex HM") as %?.
+    iDestruct (gstacks_take_out _ _ m with "Hex HM") as (s HMn) "[HM Hfl]"; first set_solver.
+    iApply (clwp_wand with "[HM Hfl HWBWP]").
+    { iApply ("HWBWP" with "[$] [$]"). }
+    iIntros (?); iDestruct 1 as (N HNM) "(Hgs & Hfl & HΦ)".
+    iDestruct (gstacks_put_back with "Hfl Hgs") as "Hgs"; first by eapply lookup_weaken; eauto.
+    replace ((out ∪ {[m]}) ∖ {[m]}) with out by set_solver.
+    iExists _; iFrame; done.
+  Qed.
+
+  Lemma wbwp_mend m s E out e Φ :
+    gstack_full m s
+    -∗ WBWP@{rs} e @ out ∖ {[m]}; E {{ Φ }}
+    -∗ WBWP@{rs} e @ out; E {{v, gstack_full m s ∗ Φ v }}.
+  Proof.
+    iIntros "Hfl HWBWP".
+    rewrite /wbwp.
+    iIntros (M) "HM".
+    iDestruct (gstack_full_is_out with "Hfl HM") as %?.
+    iDestruct (gstacks_except_included with "HM") as "%".
+    iDestruct (gstack_full_exists with "Hfl") as "#Hex".
+    destruct (M !! m) as [s'|] eqn:HMns'; last by apply not_elem_of_dom in HMns'; set_solver.
+    iDestruct (gstacks_out_swap _ _ m s with "HM") as "HM"; first done.
+    iDestruct (gstacks_put_back with "Hfl HM") as "HM"; first by rewrite lookup_insert.
+    iSpecialize ("HWBWP" with "HM").
+    iApply (clwp_wand with "[$]").
+    iIntros (?); iDestruct 1 as (N) "(%&HM&?)".
+    iDestruct (gstacks_take_out _ _ m with "Hex HM") as (s'' HMn) "[HM Hfl]"; first set_solver.
+    replace (out ∖ {[m]} ∪ {[m]}) with out; last first.
+    { apply set_eq; intros p; split; [|set_solver]. destruct (decide (m = p)); set_solver. }
+    iDestruct (gstacks_out_swap _ _ m s' with "HM") as "HM"; first done.
+    assert (N !! m = Some s).
+    { eapply lookup_weaken; last eassumption. rewrite lookup_insert //. }
+    simplify_eq /=.
+    iExists _; iFrame.
+    iPureIntro.
+    apply map_subseteq_spec.
+    intros i ? HMi.
+    destruct (decide (i = m)) as [->|]; first by rewrite HMns' in HMi; rewrite lookup_insert.
+    rewrite lookup_insert_ne //.
+    eapply lookup_weaken; last eassumption.
+    rewrite lookup_insert_ne //.
+  Qed.
+
+  Lemma wbwp_make_gstack R E out e Φ :
+    (∀ p, ⌜p ∉ out⌝
+          -∗ gstack_full p []
+          -∗ gstack_frag p [] ={E}=∗ ∃ stk, gstack_full p stk ∗ R p)
+    -∗ (∀ p, ⌜p ∉ out⌝ -∗ R p -∗ WBWP@{rs} e @ out; E {{ Φ }})
+    -∗ WBWP@{rs} e @ out; E {{ Φ }}.
+  Proof.
+    iIntros "Hstk HWP".
+    rewrite /wbwp.
+    iIntros (M) "HM".
+    iDestruct (gstacks_except_included with "HM") as %?.
+    iMod (gstack_alloc with "HM") as (m) "(%&HM&Hfr)".
+    iDestruct (gstack_frag_exists with "Hfr") as "#Hex".
+    iDestruct (gstacks_take_out with "Hex HM") as (s Hs) "[HM Hfl]"; first set_solver.
+    rewrite lookup_insert in Hs; simplify_eq.
+    iMod ("Hstk" with "[] Hfl Hfr") as (s) "[Hfl HR]"; first set_solver.
+    iDestruct (gstacks_out_swap _ _ m s with "HM") as "HM"; first set_solver.
+    iPoseProof (gstacks_put_back with "Hfl HM") as "HM"; first by rewrite lookup_insert.
+    rewrite insert_insert.
+    replace ((out ∪ {[m]}) ∖ {[m]}) with out by set_solver.
+    iApply (clwp_wand with "[-]").
+    { iApply ("HWP" with "[] [$] [$]"). set_solver. }
+    iIntros (?); iDestruct 1 as (N HNM) "(Hgs & HΦ)".
+    iExists _; iFrame.
+    iPureIntro.
+    etrans; last eassumption.
+    apply insert_subseteq, not_elem_of_dom; done.
+  Qed.
+
+  Lemma fupd_wbwp E out e Φ :
+    (|={E}=> WBWP@{rs} e @ out; E {{ Φ }}) ⊢ WBWP@{rs} e @ out; E {{ Φ }}.
+  Proof. rewrite /wbwp; iIntros "H" (M) "?"; iMod "H"; iApply "H"; iAssumption. Qed.
+  Lemma wbwp_fupd E out e (Φ : ITV -n> iProp) :
+    WBWP@{rs} e @ out; E {{ v, |={E}=> Φ v }} ⊢ WBWP@{rs} e @ out; E {{ Φ }}.
+  Proof.
+    iIntros "H".
+    iApply (wbwp_mono E with "H"); auto.
+  Qed.
+
+  Lemma wp_wbwp E out e Φ : CLWP@{rs} e @ E {{ Φ }} -∗ WBWP@{rs} e @ out; E {{ Φ }}.
+  Proof.
+    iIntros "HWP".
+    rewrite /wbwp.
+    iIntros (M) "HM".
+    iApply (clwp_wand with "HWP").
+    iIntros (?) "?"; iExists _; iFrame; done.
+  Qed.
+
+  Global Instance wbwp_bind_ne s E (κ : HOM) (Φ : ITV -n> iProp)
+    : NonExpansive (λ βv, (WBWP@{rs} (κ (IT_of_V βv)) @ s; E {{ Φ }})%I).
+  Proof.
+    solve_proper.
+  Qed.
+
+  Program Definition wbwp_bind s E (κ : HOM) e (Φ : ITV -n> iProp) :
+    WBWP@{rs} e @ s; E {{ βv, WBWP@{rs} (κ (IT_of_V βv)) @ s; E {{ Φ }} }}
+                ⊢ WBWP@{rs} (κ e) @ s; E {{ Φ }}.
+  Proof.
+    rewrite /wbwp.
+    iIntros "Hwp" (M) "HM".
+    iApply clwp_bind.
+    iApply (clwp_wand with "[Hwp HM]"); first by iApply "Hwp".
+    iIntros (?); iDestruct 1 as (?) "(%&HM&Hwp)".
+    iApply (clwp_wand with "[Hwp HM]"); first by iApply "Hwp".
+    iIntros (?); iDestruct 1 as (?) "(%&HM&Hwp)".
+    iExists _; iFrame; iPureIntro.
+    etrans; eauto.
+  Qed.
+
+  (** * Derived rules *)
+  Lemma wbwp_mono' E out e (Φ Ψ : ITV -n> iProp) :
+    (∀ v, Φ v ⊢ Ψ v)
+    → WBWP@{rs} e @ out; E {{ Φ }} ⊢ WBWP@{rs} e @ out; E {{ Ψ }}.
+  Proof.
+    iIntros (HΦ) "H"; iApply (wbwp_mono with "H"); auto.
+    iIntros (v) "?". by iApply HΦ.
+  Qed.
+
+  Lemma wbwp_frame_l E out e Φ R :
+    R ∗ WBWP@{rs} e @ out; E {{ Φ }} ⊢ WBWP@{rs} e @ out; E {{ v, R ∗ Φ v }}.
+  Proof.
+    iIntros "[? H]". iApply (wbwp_mono with "H").
+    iIntros (?) "G".
+    iModIntro.
+    iFrame.
+  Qed.
+  Lemma wbwp_frame_r E out e Φ R :
+    WBWP@{rs} e @ out; E {{ Φ }} ∗ R ⊢ WBWP@{rs} e @ out; E {{ v, Φ v ∗ R }}.
+  Proof.
+    iIntros "[H ?]". iApply (wbwp_mono with "H").
+    iIntros (?) "G".
+    iModIntro.
+    iFrame.
+  Qed.
+End wp.
+
+(** Proofmode class instances *)
+Section proofmode_classes.
+  Context {n : nat} {a : is_ctx_dep} (rs : gReifiers a n) {A} `{!Cofe A}.
+  Notation rG := (gReifiers_sReifier rs).
+  Notation F := (sReifier_ops rG).
+  Notation IT := (IT F A).
+  Notation ITV := (ITV F A).
+  Notation stateF := (gReifiers_state rs).
+  Notation stateO := (stateF ♯ IT).
+  Notation stateR := (gReifiers_ucmra rs IT).
+  Let of_state := (of_state rs IT).
+  Let of_idx := (of_idx rs IT).
+  Notation reify := (reify rG).
+  Notation istep := (istep rG).
+  Notation isteps := (isteps rG).
+  Notation sstep := (sstep rG).
+  Notation ssteps := (ssteps rG).
+
+  Implicit Type op : opid F.
+  Implicit Type α β : IT.
+
+  Context `{!invGS Σ} `{!stateG rs A Σ} `{!gstacksIG Σ}.
+  Notation iProp := (iProp Σ).
+  Notation coPsetO := (leibnizO coPset).
+
+  Global Instance frame_wbwp p E out e R (Φ Ψ : ITV -n> iProp) :
+    (∀ v, Frame p R (Φ v) (Ψ v)) →
+    Frame p R (WBWP@{rs} e @ out; E {{ Φ }}) (WBWP@{rs} e @ out; E {{ Ψ }}) | 2.
+  Proof. rewrite /Frame=> HR. rewrite wbwp_frame_l. apply wbwp_mono', HR. Qed.
+
+  Global Instance is_except_0_wbwp E out e Φ : IsExcept0 (WBWP@{rs} e @ out; E {{ Φ }}).
+  Proof. by rewrite /IsExcept0 -{2}fupd_wbwp -except_0_fupd -fupd_intro. Qed.
+
+  Global Instance elim_modal_bupd_wbwp p E out e P Φ :
+    ElimModal True p false (|==> P) P (WBWP@{rs} e @ out; E {{ Φ }}) (WBWP@{rs} e @ out; E {{ Φ }}).
+  Proof.
+    by rewrite /ElimModal intuitionistically_if_elim
+      (bupd_fupd E) fupd_frame_r wand_elim_r fupd_wbwp.
+  Qed.
+
+  Global Instance elim_modal_fupd_wbwp p E out e P Φ :
+    ElimModal True p false (|={E}=> P) P (WBWP@{rs} e @ out; E {{ Φ }}) (WBWP@{rs} e @ out; E {{ Φ }}).
+  Proof.
+    by rewrite /ElimModal intuitionistically_if_elim
+      fupd_frame_r wand_elim_r fupd_wbwp.
+  Qed.
+
+  Global Instance add_modal_fupd_wbwp E out e P Φ :
+    AddModal (|={E}=> P) P (WBWP@{rs} e @ out; E {{ Φ }}).
+  Proof. by rewrite /AddModal fupd_frame_r wand_elim_r fupd_wbwp. Qed.
+End proofmode_classes.
